Add the rr and rw versions of configurations

src/lang/ConfigurationRW.v
@@ -35,16 +35,16 @@ End Timestamps.
 
 Module Capability.
   Structure t := mk {
-    writes: Timestamps.t;
     reads: Timestamps.t;
+    writes: Timestamps.t;
   }.
 
   Definition bot: t := mk Timestamps.bot Timestamps.bot.
 
   Inductive le (lhs rhs:t): Prop :=
   | le_intro
-      (WRITES: Timestamps.le lhs.(writes) rhs.(writes))
       (READS: Timestamps.le lhs.(reads) rhs.(reads))
+      (WRITES: Timestamps.le lhs.(writes) rhs.(writes))
   .
 End Capability.
 
@@ -109,17 +109,17 @@ Module Commit.
   .
 
   Inductive read
-            (commit:t) (loc:Loc.t) (ts:positive) (ord:Ordering.t) (m:MessageSet.t)
-            (val:Const.t) (released:Capability.t) (confirmed:bool): Prop :=
+            (commit1:t) (loc:Loc.t) (ts:positive) (ord:Ordering.t) (m:MessageSet.t)
+            (commit2:t) (val:Const.t) (released:Capability.t) (confirmed:bool): Prop :=
   | read_intro
-      (COMMIT0: (Timestamps.get loc commit.(current).(Capability.reads) <= ts)%positive)
-      (COMMIT1: (ts <= Timestamps.get loc commit.(current).(Capability.writes))%positive)
+      (COMMIT0: le commit1 commit2)
+      (COMMIT1: (Timestamps.get loc commit1.(current).(Capability.reads) <= ts)%positive)
       (GET: MessageSet.get loc ts m = Some (Message.mk val released confirmed))
       (ACQUIRE: forall (ORDERING: Ordering.le Ordering.acquire ord),
-          Capability.le commit.(current) released)
-      (ACQUIRABLE: Capability.le released commit.(acquirable)):
-      read commit loc ts ord m
-           val released confirmed
+          Capability.le released commit2.(current))
+      (ACQUIRABLE: Capability.le released commit2.(acquirable)):
+      read commit1 loc ts ord m
+           commit2 val released confirmed
   .
 
   Inductive write
@@ -129,8 +129,8 @@ Module Commit.
       (DECLARE: MessageSet.get loc ts m1 = Some (Message.mk val released false))
       (COMMIT0: le commit1 commit2)
       (COMMIT1: (Timestamps.get loc commit1.(current).(Capability.writes) < ts)%positive)
-      (COMMIT2: (ts <= Timestamps.get loc commit2.(current).(Capability.writes))%positive)
-      (COMMIT3: (ts <= Timestamps.get loc commit2.(current).(Capability.reads))%positive)
+      (COMMIT2: (ts <= Timestamps.get loc commit2.(current).(Capability.reads))%positive)
+      (COMMIT3: (ts <= Timestamps.get loc commit2.(current).(Capability.writes))%positive)
       (RELEASE: forall (ORDERING: Ordering.le Ordering.release ord),
           Capability.le commit1.(current) (LocFun.find loc commit1.(Commit.released)))
       (RELEASED: Capability.le (LocFun.find loc commit1.(Commit.released)) released):
@@ -138,12 +138,15 @@ Module Commit.
             commit2 (LocFun.add loc (UsualPositiveMap.add ts (Message.mk val released true) (LocFun.find loc m1)) m1)
   .
 
-  Inductive fence (ord:Ordering.t) (th:t): Prop :=
+  Inductive fence
+            (commit1:t) (ord:Ordering.t)
+            (commit2:t): Prop :=
   | fence_intro
+      (COMMIT: le commit1 commit2)
       (ACQUIRE: forall (ORDERING: Ordering.le Ordering.acquire ord),
-          Capability.le th.(acquirable) th.(current))
+          Capability.le commit2.(acquirable) commit2.(current))
       (RELEASE: forall (ORDERING: Ordering.le Ordering.release ord) loc,
-          Capability.le th.(current) (LocFun.find loc th.(released)))
+          Capability.le commit2.(current) (LocFun.find loc commit2.(released)))
   .
 End Commit.
 
@@ -168,23 +171,24 @@ Module Configuration.
 
   (* TODO: to check the liveness, the step should be annotated with the thread id.
    *)
-  Inductive base_step (c1:t): forall (validation:option (Loc.t * positive)) (c2:t), Prop :=
+  Inductive base_step (c1:t): forall (tid:option Ident.t) (validation:option (Loc.t * positive)) (c2:t), Prop :=
   | step_tau
-      tid commit th1 th2
-      (TID: IdentMap.find tid c1.(threads) = Some (commit, th1))
+      tid commit1 commit2 th1 th2
+      (COMMIT: Commit.le commit1 commit2)
+      (TID: IdentMap.find tid c1.(threads) = Some (commit1, th1))
       (THREAD: Thread.step th1 None th2):
       base_step
-        c1 None
-        (mk c1.(messages) (IdentMap.add tid (commit, th2) c1.(threads)))
+        c1 (Some tid) None
+        (mk c1.(messages) (IdentMap.add tid (commit2, th2) c1.(threads)))
   | step_read
-      tid commit th1 th2
+      tid commit1 commit2 th1 th2
       loc ts ord val released confirmed
-      (TID: IdentMap.find tid c1.(threads) = Some (commit, th1))
-      (READ: Commit.read commit loc ts ord c1.(messages) val released confirmed)
+      (TID: IdentMap.find tid c1.(threads) = Some (commit1, th1))
+      (READ: Commit.read commit1 loc ts ord c1.(messages) commit2 val released confirmed)
       (THREAD: Thread.step th1 (Some (ThreadEvent.mem (MemEvent.read loc val ord))) th2):
       base_step
-        c1 (Some (loc, ts))
-        (mk c1.(messages) (IdentMap.add tid (commit, th2) c1.(threads)))
+        c1 (Some tid) (Some (loc, ts))
+        (mk c1.(messages) (IdentMap.add tid (commit2, th2) c1.(threads)))
   | step_write
       tid commit1 commit2 th1 th2
       loc ts ord val released messages2
@@ -192,52 +196,49 @@ Module Configuration.
       (WRITE: Commit.write commit1 loc ts val released ord c1.(messages) commit2 messages2)
       (THREAD: Thread.step th1 (Some (ThreadEvent.mem (MemEvent.write loc val ord))) th2):
       base_step
-        c1 None
+        c1 (Some tid) None
         (mk messages2 (IdentMap.add tid (commit2, th2) c1.(threads)))
   | step_update
-      tid commit1 commit2 th1 th2
+      tid commit1 commiti commit2 th1 th2
       loc ts ord valr valw releasedr releasedw confirmedr messages2
       (TID: IdentMap.find tid c1.(threads) = Some (commit1, th1))
-      (READ: Commit.read commit1 loc ts ord c1.(messages) valr releasedr confirmedr)
-      (WRITE: Commit.write commit1 loc (ts + 1) valw releasedw ord c1.(messages) commit2 messages2)
+      (READ: Commit.read commit1 loc ts ord c1.(messages) commiti valr releasedr confirmedr)
+      (WRITE: Commit.write commiti loc (ts + 1) valw releasedw ord c1.(messages) commit2 messages2)
       (RELEASE: Capability.le releasedr releasedw)
       (THREAD: Thread.step th1 (Some (ThreadEvent.mem (MemEvent.update loc valr valw ord))) th2):
       base_step
-        c1 (Some (loc, ts))
+        c1 (Some tid) (Some (loc, ts))
         (mk messages2 (IdentMap.add tid (commit2, th2) c1.(threads)))
   | step_fence
-      tid commit th1 th2
+      tid commit1 commit2 th1 th2
       ord
-      (TID: IdentMap.find tid c1.(threads) = Some (commit, th1))
-      (FENCE: Commit.fence ord commit)
+      (TID: IdentMap.find tid c1.(threads) = Some (commit1, th1))
+      (FENCE: Commit.fence commit1 ord commit2)
       (THREAD: Thread.step th1 (Some (ThreadEvent.mem (MemEvent.fence ord))) th2):
       base_step
-        c1 None
-        (mk c1.(messages) (IdentMap.add tid (commit, th2) c1.(threads)))
+        c1 (Some tid) None
+        (mk c1.(messages) (IdentMap.add tid (commit2, th2) c1.(threads)))
   | step_declare
       loc ts val released messages2
       (DECLARE: MessageSet.declare loc ts val released c1.(messages) messages2):
       base_step
-        c1 None
+        c1 None None
         (mk messages2 c1.(threads))
-  | step_commit
-      tid commit1 commit2 th
-      (TID: IdentMap.find tid c1.(threads) = Some (commit1, th))
-      (COMMIT: Commit.le commit1 commit2):
-      base_step
-        c1 None
-        (mk c1.(messages) (IdentMap.add tid (commit2, th) c1.(threads)))
   .
 
   Inductive internal_step: forall (c1 c2:t), Prop :=
   | step_confirmed
-      c1 c2
-      (STEP: base_step c1 None c2):
+      c1 c2 tid
+      (STEP: base_step c1 tid None c2):
       internal_step c1 c2
   | step_unconfirmed
-      c1 c2 loc ts
-      (STEP: base_step c1 (Some (loc, ts)) c2)
-      (VALID: valid loc ts c1):
+      c1 c2 tid loc ts
+      commit1 commit1' th1
+      (STEP: base_step c1 (Some tid) (Some (loc, ts)) c2)
+      (THREAD1: IdentMap.find tid c1.(threads) = Some (commit1, th1))
+      (COMMIT0: Commit.le commit1 commit1')
+      (COMMIT1: (ts <= commit1'.(Commit.current).(Capability.writes).(Timestamps.get loc))%positive)
+      (VALID: valid loc ts (mk c1.(messages) (IdentMap.add tid (commit1', th1) c1.(threads)))):
       internal_step c1 c2
   with valid: forall (loc:Loc.t) (ts:positive) (c1:t), Prop :=
   | valid_intro
@@ -247,36 +248,6 @@ Module Configuration.
       (NODECLARE: ~ MessageSet.declared c2.(messages) loc ts):
       valid loc ts c1
   .
-
-  Lemma internal_step_strong_ind
-        (P : t -> t -> Prop)
-        (CASE1:
-           forall c1 c2
-             (STEP: base_step c1 None c2),
-             P c1 c2)
-        (CASE2:
-           forall (c1 c2 c1' : t) (loc : Loc.t) (ts : positive)
-             (STEP: base_step c1 (Some (loc, ts)) c2)
-             (STEPS: rtc internal_step c1 c1')
-             (PROP: rtc P c1 c1')
-             (DECLARE: (MessageSet.declared (messages c1') <2= MessageSet.declared (messages c1)))
-             (NODECLARE: ~ MessageSet.declared (messages c1') loc ts),
-             P c1 c2)
-        c1 c2
-        (STEP: internal_step c1 c2):
-    P c1 c2.
-  Proof.
-    revert c1 c2 STEP. fix IH 3. intros c1 c2 H. inv H.
-    - apply CASE1. auto.
-    - inv VALID. eapply CASE2.
-      + eauto.
-      + eauto.
-      + clear -IH STEPS.
-        induction STEPS; eauto.
-        econs 2; eauto.
-      + eauto.
-      + eauto.
-  Qed.
 
   Inductive consistent: forall (c1:t), Prop :=
   | consistent_intro
