src/lang/ConfigurationRR.v
@@ -1,0 +1,337 @@
+Require Import List.
+Require Import Equalities.
+Require Import PeanoNat.
+Require Import Relations.
+Require Import MSetList.
+Require Import Omega.
+
+Require Import sflib.
+Require Import paco.
+
+Require Import DataStructure.
+Require Import Basic.
+Require Import Event.
+Require Import Thread.
+Require Import UsualFMapPositive.
+
+Set Implicit Arguments.
+Import ListNotations.
+
+
+(* TODO: how about using functor in defining structures with bot/le?
+ *)
+Module Timestamps.
+  Definition t := LocFun.t positive.
+
+  Definition bot: t := LocFun.init 1%positive.
+
+  Definition le (lhs rhs:t): Prop :=
+    forall loc, (LocFun.find loc lhs <= LocFun.find loc rhs)%positive.
+
+  Definition get (loc:Loc.t) (c:t) :=
+    LocFun.find loc c.
+End Timestamps.
+
+
+Module Capability.
+  Structure t := mk {
+    lb: Timestamps.t;
+    ub: Timestamps.t;
+  }.
+
+  Definition bot: t := mk Timestamps.bot Timestamps.bot.
+
+  Inductive le (lhs rhs:t): Prop :=
+  | le_intro
+      (LB: Timestamps.le lhs.(lb) rhs.(lb))
+      (UB: Timestamps.le lhs.(ub) rhs.(ub))
+  .
+End Capability.
+
+
+Module Message.
+  Structure t := mk {
+    val: Const.t;
+    released: Capability.t;
+    confirmed: bool;
+  }.
+End Message.
+
+
+Module MessageSet.
+  Definition t := LocFun.t (UsualPositiveMap.t Message.t).
+
+  Definition init: t :=
+    LocFun.init
+      (UsualPositiveMap.add
+         1%positive
+         (Message.mk 0 Capability.bot true)
+         (UsualPositiveMap.empty _)).
+
+  Definition get (loc:Loc.t) (ts:positive) (m:t): option Message.t :=
+    UsualPositiveMap.find ts (LocFun.find loc m).
+
+  Inductive declare (loc:Loc.t) (ts:positive) (val:Const.t) (released:Capability.t) (m1:t): forall (m2:t), Prop :=
+  | declare_intro
+      (GET: get loc ts m1 = None):
+      declare loc ts val released m1
+              (LocFun.add loc (UsualPositiveMap.add ts (Message.mk val released false) (LocFun.find loc m1)) m1)
+  .
+
+  Inductive declared (m:t) (loc:Loc.t) (ts:positive): Prop :=
+  | declared_intro
+      val released
+      (GET: MessageSet.get loc ts m = Some (Message.mk val released false))
+  .
+
+  Inductive confirmed (m:t): Prop :=
+  | confirmed_intro
+      (CONFIRM: forall loc ts, ~ declared m loc ts)
+  .
+End MessageSet.
+
+
+Module Commit.
+  Structure t := mk {
+    current: Capability.t;
+    released: LocFun.t Capability.t;
+    acquirable: Capability.t;
+  }.
+
+  Definition bot: t :=
+    mk Capability.bot (LocFun.init Capability.bot) Capability.bot.
+
+  Inductive le (lhs rhs:t): Prop :=
+  | le_intro
+      (CURRENT: Capability.le lhs.(current) rhs.(current))
+      (RELEASED: forall (loc:Loc.t), Capability.le (LocFun.find loc lhs.(released)) (LocFun.find loc rhs.(released)))
+      (ACQUIRABLE: Capability.le lhs.(acquirable) rhs.(acquirable))
+  .
+
+  Inductive read
+            (commit:t) (loc:Loc.t) (ts:positive) (ord:Ordering.t) (m:MessageSet.t)
+            (val:Const.t) (released:Capability.t) (confirmed:bool): Prop :=
+  | read_intro
+      (COMMIT0: (Timestamps.get loc commit.(current).(Capability.lb) <= ts)%positive)
+      (COMMIT1: (ts <= Timestamps.get loc commit.(current).(Capability.ub))%positive)
+      (GET: MessageSet.get loc ts m = Some (Message.mk val released confirmed))
+      (ACQUIRE: forall (ORDERING: Ordering.le Ordering.acquire ord),
+          Capability.le released commit.(current))
+      (ACQUIRABLE: Capability.le released commit.(acquirable)):
+      read commit loc ts ord m
+           val released confirmed
+  .
+
+  Inductive write
+            (commit1:t) (loc:Loc.t) (ts:positive) (val:Const.t) (released:Capability.t) (ord:Ordering.t) (m1:MessageSet.t)
+            (commit2:t): forall (m2:MessageSet.t), Prop :=
+  | write_intro
+      (DECLARE: MessageSet.get loc ts m1 = Some (Message.mk val released false))
+      (COMMIT0: le commit1 commit2)
+      (COMMIT1: (Timestamps.get loc commit1.(current).(Capability.ub) < ts)%positive)
+      (COMMIT2: (ts <= Timestamps.get loc commit2.(current).(Capability.lb))%positive)
+      (COMMIT3: (ts <= Timestamps.get loc commit2.(current).(Capability.ub))%positive)
+      (RELEASE: forall (ORDERING: Ordering.le Ordering.release ord),
+          Capability.le commit1.(current) (LocFun.find loc commit1.(Commit.released)))
+      (RELEASED: Capability.le (LocFun.find loc commit1.(Commit.released)) released):
+      write commit1 loc ts val released ord m1
+            commit2 (LocFun.add loc (UsualPositiveMap.add ts (Message.mk val released true) (LocFun.find loc m1)) m1)
+  .
+
+  Inductive fence (commit:t) (ord:Ordering.t): Prop :=
+  | fence_intro
+      (ACQUIRE: forall (ORDERING: Ordering.le Ordering.acquire ord),
+          Capability.le commit.(acquirable) commit.(current))
+      (RELEASE: forall (ORDERING: Ordering.le Ordering.release ord) loc,
+          Capability.le commit.(current) (LocFun.find loc commit.(released)))
+  .
+End Commit.
+
+
+Module Configuration.
+  Definition syntax := IdentMap.t Thread.syntax.
+
+  Structure t := mk {
+    messages: MessageSet.t;
+    threads: IdentMap.t (Commit.t * Thread.t);
+  }.
+
+  Definition init (s:syntax): t :=
+    mk MessageSet.init (IdentMap.map (fun th => (Commit.bot, Thread.init th)) s).
+
+  Inductive is_terminal (c:t): Prop :=
+  | is_terminal_intro
+      (TERMINAL:
+         forall tid commit th (FIND: IdentMap.find tid c.(threads) = Some (commit, th)),
+           Thread.is_terminal th)
+  .
+
+  (* TODO: to check the liveness, the step should be annotated with the thread id.
+   *)
+  Inductive base_step (c1:t): forall (validation:option (Loc.t * positive)) (c2:t), Prop :=
+  | step_tau
+      tid commit th1 th2
+      (TID: IdentMap.find tid c1.(threads) = Some (commit, th1))
+      (THREAD: Thread.step th1 None th2):
+      base_step
+        c1 None
+        (mk c1.(messages) (IdentMap.add tid (commit, th2) c1.(threads)))
+  | step_read
+      tid commit th1 th2
+      loc ts ord val released confirmed
+      (TID: IdentMap.find tid c1.(threads) = Some (commit, th1))
+      (READ: Commit.read commit loc ts ord c1.(messages) val released confirmed)
+      (THREAD: Thread.step th1 (Some (ThreadEvent.mem (MemEvent.read loc val ord))) th2):
+      base_step
+        c1 (Some (loc, ts))
+        (mk c1.(messages) (IdentMap.add tid (commit, th2) c1.(threads)))
+  | step_write
+      tid commit1 commit2 th1 th2
+      loc ts ord val released messages2
+      (TID: IdentMap.find tid c1.(threads) = Some (commit1, th1))
+      (WRITE: Commit.write commit1 loc ts val released ord c1.(messages) commit2 messages2)
+      (THREAD: Thread.step th1 (Some (ThreadEvent.mem (MemEvent.write loc val ord))) th2):
+      base_step
+        c1 None
+        (mk messages2 (IdentMap.add tid (commit2, th2) c1.(threads)))
+  | step_update
+      tid commit1 commit2 th1 th2
+      loc ts ord valr valw releasedr releasedw confirmedr messages2
+      (TID: IdentMap.find tid c1.(threads) = Some (commit1, th1))
+      (READ: Commit.read commit1 loc ts ord c1.(messages) valr releasedr confirmedr)
+      (WRITE: Commit.write commit1 loc (ts + 1) valw releasedw ord c1.(messages) commit2 messages2)
+      (RELEASE: Capability.le releasedr releasedw)
+      (THREAD: Thread.step th1 (Some (ThreadEvent.mem (MemEvent.update loc valr valw ord))) th2):
+      base_step
+        c1 (Some (loc, ts))
+        (mk messages2 (IdentMap.add tid (commit2, th2) c1.(threads)))
+  | step_fence
+      tid commit th1 th2
+      ord
+      (TID: IdentMap.find tid c1.(threads) = Some (commit, th1))
+      (FENCE: Commit.fence commit ord)
+      (THREAD: Thread.step th1 (Some (ThreadEvent.mem (MemEvent.fence ord))) th2):
+      base_step
+        c1 None
+        (mk c1.(messages) (IdentMap.add tid (commit, th2) c1.(threads)))
+  | step_declare
+      loc ts val released messages2
+      (DECLARE: MessageSet.declare loc ts val released c1.(messages) messages2):
+      base_step
+        c1 None
+        (mk messages2 c1.(threads))
+  | step_commit
+      tid commit1 commit2 th
+      (TID: IdentMap.find tid c1.(threads) = Some (commit1, th))
+      (COMMIT: Commit.le commit1 commit2):
+      base_step
+        c1 None
+        (mk c1.(messages) (IdentMap.add tid (commit2, th) c1.(threads)))
+  .
+
+  Inductive internal_step: forall (c1 c2:t), Prop :=
+  | step_confirmed
+      c1 c2
+      (STEP: base_step c1 None c2):
+      internal_step c1 c2
+  | step_unconfirmed
+      c1 c2 loc ts
+      (STEP: base_step c1 (Some (loc, ts)) c2)
+      (VALID: valid loc ts c1):
+      internal_step c1 c2
+  with valid: forall (loc:Loc.t) (ts:positive) (c1:t), Prop :=
+  | valid_intro
+      c1 c2 loc ts
+      (STEPS: rtc internal_step c1 c2)
+      (DECLARE: MessageSet.declared c2.(messages) <2= MessageSet.declared c1.(messages))
+      (NODECLARE: ~ MessageSet.declared c2.(messages) loc ts):
+      valid loc ts c1
+  .
+
+  Lemma internal_step_strong_ind
+        (P : t -> t -> Prop)
+        (CASE1:
+           forall c1 c2
+             (STEP: base_step c1 None c2),
+             P c1 c2)
+        (CASE2:
+           forall (c1 c2 c1' : t) (loc : Loc.t) (ts : positive)
+             (STEP: base_step c1 (Some (loc, ts)) c2)
+             (STEPS: rtc internal_step c1 c1')
+             (PROP: rtc P c1 c1')
+             (DECLARE: (MessageSet.declared (messages c1') <2= MessageSet.declared (messages c1)))
+             (NODECLARE: ~ MessageSet.declared (messages c1') loc ts),
+             P c1 c2)
+        c1 c2
+        (STEP: internal_step c1 c2):
+    P c1 c2.
+  Proof.
+    revert c1 c2 STEP. fix IH 3. intros c1 c2 H. inv H.
+    - apply CASE1. auto.
+    - inv VALID. eapply CASE2.
+      + eauto.
+      + eauto.
+      + clear -IH STEPS.
+        induction STEPS; eauto.
+        econs 2; eauto.
+      + eauto.
+      + eauto.
+  Qed.
+
+  Inductive consistent: forall (c1:t), Prop :=
+  | consistent_intro
+      c1 c2
+      (STEPS: rtc internal_step c1 c2)
+      (CONFIRM: MessageSet.confirmed c2.(messages)):
+      consistent c1
+  .
+
+  Lemma internal_steps_consistent c1 c2
+        (STEPS: rtc internal_step c1 c2)
+        (CONSISTENT: consistent c2):
+    consistent c1.
+  Proof.
+    inv CONSISTENT. econs; [|eauto].
+    eapply rtc_trans; eauto.
+  Qed.
+
+  Lemma init_consistent s: consistent (init s).
+  Proof.
+    econs.
+    - econs 1.
+    - unfold init. simpl. econs. i. intro X. inv X.
+      unfold MessageSet.get, MessageSet.init in *.
+      rewrite LocFun.init_spec in *.
+      rewrite IdentMap.Facts.add_o in *.
+      match goal with
+      | [H: context[if ?cond then _ else _] |- _] =>
+        destruct cond; inv H
+      end.
+      rewrite IdentMap.Facts.empty_o in *. inv H0.
+  Qed.
+
+  Inductive external_step (c1:t): forall (e:Event.t) (c2:t), Prop :=
+  | step_syscall
+      tid commit th1 th2
+      e
+      (TID: IdentMap.find tid c1.(threads) = Some (commit, th1))
+      (THREAD: Thread.step th1 (Some (ThreadEvent.syscall e)) th2):
+      external_step
+        c1 e
+        (mk c1.(messages) (IdentMap.add tid (commit, th2) c1.(threads)))
+  .
+
+  Inductive step: forall (c1:t) (e:option Event.t) (c2:t), Prop :=
+  | step_internal
+      c1 c2
+      (STEP: internal_step c1 c2)
+      (CONSISTENT: consistent c2):
+      step c1 None c2
+  | step_external
+      c1 c2
+      e
+      (STEP: external_step c1 e c2)
+      (CONSISTENT: consistent c2):
+      step c1 (Some e) c2
+  .
+End Configuration.
