src/opt/Reorder.v
@@ -1,7 +1,6 @@
 Require Import Basics.
 Require Import Bool.
 Require Import List.
-Require Import ProofIrrelevance.
 
 Require Import sflib.
 Require Import paco.
@@ -9,7 +8,7 @@ Require Import paco.
 Require Import Basic.
 Require Import Event.
 Require Import Thread.
-Require Import Configuration.
+Require Import ConfigurationRR.
 Require Import Simulation.
 Require Import Syntax.
 Require Import Semantics.
